use Coq 8.17

Keys.v
@@ -4,6 +4,7 @@ Require Import Coq.Structures.OrderedType.
 Require Import Coq.Structures.DecidableTypeEx.
 Require Import Coq.ZArith.Znat.
 Require Import Coq.Arith.Peano_dec.
+Require Import Coq.Arith.PeanoNat.
 
 Module Type IndexedType.
   Variable t: Type.
@@ -15,9 +16,9 @@ End IndexedType.
 
 Module IndexedAscii <: IndexedType.
 
-Definition t := ascii.
-Definition index := nat_of_ascii.
-Definition eq := ascii_dec.
+Global Definition t := ascii.
+Global Definition index := nat_of_ascii.
+Global Definition eq := ascii_dec.
 Hypothesis index_inj: forall (x y: t), index x = index y <-> x = y.
 
 End IndexedAscii.
@@ -43,13 +44,13 @@ Qed.
 Lemma lt_not_eq : forall x y : t, lt x y -> ~ eq x y.
 Proof.
   unfold lt; unfold eq; intros.
-  red. intro. subst y. generalize dependent H. apply lt_irrefl.
+  red. intro. subst y. generalize dependent H. apply Nat.lt_irrefl.
 Qed.
 
 Lemma compare : forall x y : t, Compare lt eq x y.
 Proof.
   intros. 
-  case_eq ( nat_compare (A.index x) (A.index y)); intro.
+  case_eq ( Nat.compare (A.index x) (A.index y)); intro.
   - apply EQ. apply nat_compare_eq in H. apply A.index_inj. assumption.
   - apply LT. apply nat_compare_lt in H. unfold lt. assumption.
   - apply GT. apply nat_compare_gt in H. unfold lt. intuition.
@@ -57,12 +58,13 @@ Qed.
 
 Lemma eq_dec : forall x y, { eq x y } + { ~ eq x y }.
 Proof.
-  intros. case_eq (nat_compare (A.index x) (A.index y)); intros.
+  intros. case_eq (Nat.compare (A.index x) (A.index y)); intros.
   - left. apply nat_compare_eq in H. apply A.index_inj. assumption.
-  - right. red. intro. inversion H0. apply nat_compare_lt in H. apply A.index_inj in H1. 
-    intuition.
+  - right. red. intro. inversion H0. apply nat_compare_Lt_lt in H. apply A.index_inj in H1. 
+    rewrite H1 in H. generalize dependent H. apply Nat.lt_irrefl.
   - right. red. intro. inversion H0. apply nat_compare_gt in H. apply A.index_inj in H1. 
-    intuition.
+    rewrite H1 in H.
+    generalize dependent H. apply Nat.lt_irrefl.
 Defined.
 
 End OrderedAscii.
