Heap.v
@@ -4,7 +4,6 @@ Require Import Coq.FSets.FMapAVL.
 Require Import Coq.Program.Equality.
 Require Import Coq.Logic.FunctionalExtensionality.
 
-Add LoadPath "." as Top0.
 Require Import Top0.Tactics.
 Require Import Top0.Definitions.
 Require Import Top0.Keys.
