TypeSystem.v
@@ -6,7 +6,6 @@ Require Import Ascii.
 Require Import Coq.ZArith.Znat.
 Require Import Coq.Program.Equality.
 
-Add LoadPath "." as Top0.
 Require Import Top0.Tactics.
 Require Import Top0.Keys.
 Require Import Top0.Definitions.
@@ -18,7 +17,6 @@ Require Import Top0.Heap.
 Require Import Top0.Determinism.
 Require Import Top0.Axioms.
 
-Require Import Omega.
 
 Module TypeSoundness.
 
@@ -256,27 +254,27 @@ Proof.
   dynamic_cases (dependent induction D) Case;
   intros stty ctxt rgns t static_eff Hhp Hrho Henv Hexp; 
   inversion Hexp; subst.   
-  Case "cnt n".
-    exists stty; (split; [| split]; auto). rewrite subst_rho_natural.
+  (* Case_str "cnt n". *)
+  - exists stty; (split; [| split]; auto). rewrite subst_rho_natural.
     econstructor; eassumption.
-  Case "bool b".
-    exists stty;  (split; [| split]; auto). rewrite subst_rho_boolean.
+  (* Case "bool b". *)
+  -  exists stty;  (split; [| split]; auto). rewrite subst_rho_boolean.
     econstructor; eassumption. 
-  Case "var x".
-    exists stty; (split; [| split]; auto).
+  (* Case "var x". *)
+  -  exists stty; (split; [| split]; auto).
     eapply ty_sound_var; eassumption. 
-  Case "mu_abs". 
-    exists stty; (split; [| split]; auto).
+  (* Case "mu_abs". *)
+  - exists stty; (split; [| split]; auto).
     eapply ty_sound_closure; try (solve [eassumption]). auto.
     assert (TcInc (ctxt, rgns)) by admit.
     auto.
-  Case "rgn_abs". 
-    exists stty;  (split; [| split]; auto). 
+  (* Case "rgn_abs". *)
+  -  exists stty;  (split; [| split]; auto). 
     eapply ty_sound_region_closure; try (solve [eassumption]). auto.
     assert (TcInc (ctxt, rgns)) by admit.
     auto.
-  Case "mu_app".   
-    edestruct IHD1 as [sttym [Weak1 [TcHeap1 TcVal_mu]]]; eauto. 
+  (* Case "mu_app". *)
+  - edestruct IHD1 as [sttym [Weak1 [TcHeap1 TcVal_mu]]]; eauto. 
     edestruct IHD2 as [sttya [Weaka [TcHeapa TcVal_arg]]]; eauto.  
     eapply ext_stores__env; eauto.  
     inversion TcVal_mu as [ | | | ? ? ? ? ? ? ? ?  TcRho_rho' TcEnv_env' TcExp_abs | | |] ; subst.      
@@ -288,71 +286,73 @@ Proof.
     rewrite <- SubstEq1 in TcVal_arg.
     unfold update_rec_E, update_rec_T in *. 
     edestruct IHD3 as [sttyb [Weakb [TcHeapb TcVal_res]]]; eauto.
-    SCase "TcEnv". 
-     apply update_env. apply update_env. eapply ext_stores__env; eauto.  
-     eapply ext_stores__val; eauto. eassumption.
-     exists sttyb; intuition.  
-  Case "rgn_app".     
-    edestruct IHD1 as [sttyl [Weak1 [TcHeap1 TcVal_lam]]]; eauto. 
-    inversion TcVal_lam as  [ | | | ? ? ? ? ? ? ?  TcRho_rho' TcInc'  TcEnv_env' TcExp_lam | | |]; subst.   
-    inversion TcExp_lam as [ | | | | ? ? ? ? ? ? ? ? ? TcExp_eb | | | | | | | | | | | | | | | | | | | |  ]; subst.  
-    edestruct IHD2 as [sttyr [Weak2 [TcHeap2 TcVal_res]]]; eauto using update_env, ext_stores__env.
-    apply update_rho. assumption. assumption. eapply extended_rho; eauto. 
-    exists sttyr; intuition. 
-    rewrite subst_rho_forallrgn in H5.
-    rewrite subst_rho_forallrgn in H5.
-    inversion H5.  
-    unfold update_R in TcVal_res. 
-    simpl in TcVal_res. rewrite subst_add_comm in TcVal_res.
-    SCase "abstraction body is well typed".
-    unfold subst_in_type in TcVal_res.
-    rewrite SUBST_AS_CLOSE_OPEN in TcVal_res; auto.
-    erewrite subst_rho_open_close in TcVal_res; eauto. 
-    SCase "bound variable is free".
-    eapply bound_var_is_fresh; eauto.
-  Case "eff_app".
-    edestruct IHD1 as [sttym [Weak1 [TcHeap1 TcVal_mu]]]; eauto.
+    (* SCase "TcEnv". *)    
+    + apply update_env. apply update_env. eapply ext_stores__env; eauto.  
+      eapply ext_stores__val; eauto. eassumption.
+    + exists sttyb; intuition.  
+    (* SCase "TcVal". *)
+    - edestruct IHD1 as [sttyl [Weak1 [TcHeap1 TcVal_lam]]]; eauto. 
+      inversion TcVal_lam as  [ | | | ? ? ? ? ? ? ?  TcRho_rho' TcInc'  TcEnv_env' TcExp_lam | | |]; subst.   
+      inversion TcExp_lam as [ | | | | ? ? ? ? ? ? ? ? ? TcExp_eb | | | | | | | | | | | | | | | | | | | |  ]; subst.  
+      edestruct IHD2 as [sttyr [Weak2 [TcHeap2 TcVal_res]]]; eauto using update_env, ext_stores__env.
+      apply update_rho. assumption. assumption. eapply extended_rho; eauto. 
+      exists sttyr; intuition. 
+      rewrite subst_rho_forallrgn in H5.
+      rewrite subst_rho_forallrgn in H5.
+      inversion H5.  
+      unfold update_R in TcVal_res. 
+      simpl in TcVal_res. rewrite subst_add_comm in TcVal_res.
+      (* SCase "abstraction body is well typed". *)
+      + unfold subst_in_type in TcVal_res.
+      rewrite SUBST_AS_CLOSE_OPEN in TcVal_res; auto.
+      erewrite subst_rho_open_close in TcVal_res; eauto. 
+      (* SCase "bound variable is free". *)      
+      +  eapply bound_var_is_fresh; eauto.
+  (* Case "eff_app". *)
+  - edestruct IHD1 as [sttym [Weak1 [TcHeap1 TcVal_mu]]]; eauto.
     edestruct IHD2 as [sttya [Weaka [TcHeapa TcVal_arg]]]; eauto using ext_stores__env.
     inversion TcVal_mu as  [ | | | ? ? ? ? ? ? ? TcRho_rho' TcInc' TcEnv_env' TcExp_abs | | |]; subst. 
     inversion TcExp_abs as [ | | | | ? ? ? ? ? ? ? ? ? TcExp_eb | | | | | | | | | | | | | | | | | | | |  ]; subst. 
     edestruct IHD3 as [sttyb [Weakb [TcHeapb TcVal_res]]]; eauto.
-    SCase "Extended Env".
-      apply update_env.
-      SSCase "TcEnv". apply update_env.
-        SSSCase "Extended". eapply ext_stores__env; eauto.
-        SSSCase "Extended TcVal". rewrite <- H4 in TcVal_mu.  eapply ext_stores__val; eauto.
-      SSCase "TcVal". do 2 rewrite subst_rho_arrow in H4.
-          inversion H4.
-          assert (SubstEq: subst_rho rho' tyx = subst_rho rho tya) by assumption.
-          rewrite <- SubstEq in TcVal_arg.  eassumption. 
-    exists sttyb. intuition.
+    (* SCase "Extended Env". *)
+    + apply update_env.
+      (* SSCase "TcEnv". *)
+      * { apply update_env.
+          (* SSSCase "Extended". *)
+          - eapply ext_stores__env; eauto.
+          (* SSSCase "Extended TcVal". *)          
+         - rewrite <- H4 in TcVal_mu.  eapply ext_stores__val; eauto. }
+      (* SSCase "TcVal". *)       
+      * do 2 rewrite subst_rho_arrow in H4.
+        inversion H4.
+        assert (SubstEq: subst_rho rho' tyx = subst_rho rho tya) by assumption.
+        rewrite <- SubstEq in TcVal_arg.  eassumption. 
+    + exists sttyb. intuition.
     rewrite subst_rho_effect. rewrite subst_rho_effect in TcVal_res.
     assumption.
-  Case "par_pair". 
-    edestruct IHD3 as [sttym [Weak1 [TcHeap1 TcVal_app1]]]; eauto. 
+  (* Case "par_pair". *)
+  - edestruct IHD3 as [sttym [Weak1 [TcHeap1 TcVal_app1]]]; eauto. 
     edestruct IHD4 as [sttya [Weaka [TcHeapa TcVal_app2]]]; eauto. 
-    (*inversion TcVal_app1 as [A B [C D HRApp1] | | | | | |]; subst. 
-    inversion TcVal_app2 as [A B [C D HRApp2] | | | | | |]; subst.*)  
     exists (Functional_Map_Union sttya sttym). intuition. 
-    SCase "Weakening". 
-      apply UnionStoreTyping; [apply Weaka | apply Weak1]; auto.
-    SCase "TcHeap".
-      eapply UnionTcHeap with (theta1:=theta1) (theta2:=theta2); eauto.  
-    SCase "TcVal".
-      rewrite subst_rho_pair. 
+    (* SCase "Weakening". *)
+    + apply UnionStoreTyping; [apply Weaka | apply Weak1]; auto.
+    (* SCase "TcHeap". *)
+    + eapply UnionTcHeap with (theta1:=theta1) (theta2:=theta2); eauto.  
+    (* SCase "TcVal". *)
+    + rewrite subst_rho_pair. 
       econstructor; [eapply TcValExtended_2 | eapply TcValExtended_1]; eauto.
-  Case "cond_true".  
-    edestruct IHD1 as [sttyb [Weakb [TcHeapvb TcVal_e0]]]; eauto. 
+  (* Case "cond_true". *)
+  - edestruct IHD1 as [sttyb [Weakb [TcHeapvb TcVal_e0]]]; eauto. 
     edestruct IHD2 as [stty1 [Weak1 [TcHeapv1 TcVal_e1]]]; 
       eauto using ext_stores__env.
     exists stty1. intuition.
-  Case "cond_false".
-    edestruct IHD1 as [sttyb [Weakb [TcHeapvb TcVal_e0]]]; eauto. 
+  (* Case "cond_false". *)
+  - edestruct IHD1 as [sttyb [Weakb [TcHeapvb TcVal_e0]]]; eauto. 
     edestruct IHD2 as [stty2 [Weak2 [TcHeapv2 TcVal_e2]]]; 
       eauto using ext_stores__env.
     exists stty2. intuition.  
-  Case "new_ref e".          
-    edestruct IHD with (stty := stty)
+  (* Case "new_ref e". *)
+  - edestruct IHD with (stty := stty)
                       (ctxt := ctxt)
                       (rgns := rgns)  
                       (t := t0)
@@ -361,39 +361,39 @@ Proof.
     assert (find_H (r, allocate_H heap' r) heap' = None)
       by (apply allocate_H_fresh).
     exists (update_ST ((r, allocate_H heap' r), subst_rho rho t0) sttyv); split; [ | split].  
-    SCase "Extended stores".   
-      intros k' t' STfind. destruct k' as [r' l']. 
+    (* SCase "Extended stores". *)
+    + intros k' t' STfind. destruct k' as [r' l']. 
       destruct (eq_nat_dec r r'); destruct (eq_nat_dec (allocate_H heap' r) l'); subst. 
-      SSCase "New address must be fresh, prove by contradiction".
-        apply Weakv in STfind. 
+      (* SSCase "New address must be fresh, prove by contradiction". *)
+      * apply Weakv in STfind. 
         inversion_clear TcHeapv as [? ? ?  STfind_Hfind ?].  
         destruct (STfind_Hfind (r', allocate_H heap' r') t' STfind) as [x F].
         assert (C : None = Some x) by (rewrite <- F; rewrite <- H0; reflexivity).
         discriminate. 
-      SSCase "Existing addresses are well-typed 1".
-        apply ST_diff_key_2; [ simpl; intuition; apply n; congruence | now apply Weakv in STfind ].
-      SSCase "Existing addresses are well-typed 2".
-        apply ST_diff_key_2; [ simpl; intuition; apply n; congruence | now apply Weakv in STfind ].
-      SSCase "Existing addresses are well-typed 3".
-        apply ST_diff_key_2; [simpl; intuition; apply n; congruence | now apply Weakv ].
-    SCase "Heap typeness".  
-      apply update_heap_fresh; eauto. 
+      (* SSCase "Existing addresses are well-typed 1". *)
+      * apply ST_diff_key_2; [ simpl; intuition; apply n; congruence | now apply Weakv in STfind ].
+      (*SSCase "Existing addresses are well-typed 2". *)
+      * apply ST_diff_key_2; [ simpl; intuition; apply n; congruence | now apply Weakv in STfind ].
+      (* SSCase "Existing addresses are well-typed 3". *)
+      * apply ST_diff_key_2; [simpl; intuition; apply n; congruence | now apply Weakv ].
+    (* SCase "Heap typeness". *)
+    + apply update_heap_fresh; eauto. 
       remember (find_ST (r, allocate_H heap' r) sttyv) as to; symmetry in Heqto.
       destruct to as [ t | ]. 
-      SSCase "New address must be fresh, prove by contradiction".
-        inversion_clear TcHeapv as [? ? ? STfind_Hfind ?].  
+      (* SSCase "New address must be fresh, prove by contradiction". *)
+      * inversion_clear TcHeapv as [? ? ? STfind_Hfind ?].  
         destruct (STfind_Hfind (r, allocate_H heap' r) t Heqto) as [? ex].
         rewrite H0 in ex. discriminate.
-      SSCase "Heap typeness is preserved".
-         reflexivity. 
-    SCase "Loc is well-typed".
-       simpl in H; inversion H; subst. 
-       rewrite subst_rho_tyref. unfold mk_rgn_type. rewrite subst_rho_rgn_const.
-       econstructor. apply ST_same_key_1.
-       intro.
-       eapply TcVal_implies_closed in TcVal_v; eauto.
-  Case "get_ref e".    
-    edestruct IHD with (hp'0 := hp')
+      (* SSCase "Heap typeness is preserved". *)
+      * reflexivity. 
+    (* SCase "Loc is well-typed". *)
+    + simpl in H; inversion H; subst. 
+      rewrite subst_rho_tyref. unfold mk_rgn_type. rewrite subst_rho_rgn_const.
+      econstructor. apply ST_same_key_1.
+      intro.
+      eapply TcVal_implies_closed in TcVal_v; eauto.
+  (* Case "get_ref e". *)
+  - edestruct IHD with (hp' := hp')
                       (v := Loc (Rgn2_Const true false s) l) 
                       (stty := stty)
                       (rgns := rgns)
@@ -403,17 +403,17 @@ Proof.
                       (dynamic_eff := aacts)
     as [sttyv [Weakv [TcHeapv TcVal_v]]]; eauto.
     exists sttyv. split; [ | split].
-    SCase "HeapTyping extends".
-      apply Weakv.
-    SCase "Heap is well typed".
-      apply TcHeapv.
-    SCase "Value is well-typed". 
-      inversion_clear TcHeapv as [? ? ? ? HeapTcVal]. eapply HeapTcVal; eauto. 
+    (* SCase "HeapTyping extends". *)
+    + apply Weakv.
+    (* SCase "Heap is well typed". *)
+    + apply TcHeapv.
+    (* SCase "Value is well-typed". *) 
+    + inversion_clear TcHeapv as [? ? ? ? HeapTcVal]. eapply HeapTcVal; eauto. 
       inversion TcVal_v; subst; simpl in H; inversion H; subst.
       rewrite subst_rho_tyref in H7. inversion H7. subst.
       assumption.
-  Case "set_ref e1 e2".  
-    edestruct IHD1 with (hp' := heap')
+  (* Case "set_ref e1 e2". *)
+  - edestruct IHD1 with (hp' := heap')
                        (v := Loc (Rgn2_Const true false s) l) 
                        (stty := stty)
                        (ctxt := ctxt)
@@ -429,55 +429,58 @@ Proof.
                        (static_eff := veff)
       as [sttyv [Weakv [TcHeapv TcVal_v]]]; eauto using ext_stores__env.
     exists sttyv. split; [ | split].
-    SCase "HeapTyping extends".
-      eapply weakening_trans; eauto.
-    SCase "New heap is well typed". 
-      apply update_heap_exists with (t:= subst_rho rho t0).   
+    (* SCase "HeapTyping extends". *)
+    + eapply weakening_trans; eauto.
+    (* SCase "New heap is well typed". *)
+    + apply update_heap_exists with (t:= subst_rho rho t0).   
       { assumption. }
       { apply Weakv. inversion TcVal_a; subst. 
         simpl in H; inversion H; subst.
         rewrite subst_rho_tyref in H4. inversion H4. subst.
         assumption. }
       { assumption. }
-    SCase "Result value is well-typed".
-      rewrite subst_rho_unit. constructor.
-  Case "nat_plus x y". 
-    edestruct IHD1 as [sttyx [Weakx [TcHeapvx TcVal_x]]]; eauto. 
+    (* SCase "Result value is well-typed". *)
+    + rewrite subst_rho_unit. constructor.
+  (* Case "nat_plus x y". *)
+  - edestruct IHD1 as [sttyx [Weakx [TcHeapvx TcVal_x]]]; eauto. 
     edestruct IHD2 as [sttyy [Weaky [TcHeapvy TcVal_y]]]; 
       eauto using ext_stores__env. 
     exists sttyy. intuition. rewrite subst_rho_natural. constructor.
-  Case "nat_minus x y". 
-    edestruct IHD1 as [sttyx [Weakx [TcHeapvx TcVal_x]]]; eauto. 
+  (* Case "nat_minus x y". *)
+  - edestruct IHD1 as [sttyx [Weakx [TcHeapvx TcVal_x]]]; eauto. 
     edestruct IHD2 as [sttyy [Weaky [TcHeapvy TcVal_y]]]; 
       eauto using ext_stores__env.
     exists sttyy. intuition. rewrite subst_rho_natural. constructor.
-  Case "nat_times x y". 
-    edestruct IHD1 as [sttyx [Weakx [TcHeapvx TcVal_x]]]; eauto. 
+  (* Case "nat_times x y". *)
+  - edestruct IHD1 as [sttyx [Weakx [TcHeapvx TcVal_x]]]; eauto. 
     edestruct IHD2 as [sttyy [Weaky [TcHeapvy TcVal_y]]]; 
       eauto using ext_stores__env.
     exists sttyy. intuition. rewrite subst_rho_natural. constructor.
-  Case "bool_eq x y". 
-    edestruct IHD1 as [sttyx [Weakx [TcHeapvx TcVal_x]]]; eauto. 
+  (* Case "bool_eq x y". *)
+  -  edestruct IHD1 as [sttyx [Weakx [TcHeapvx TcVal_x]]]; eauto. 
     edestruct IHD2 as [sttyy [Weaky [TcHeapvy TcVal_y]]]; 
       eauto using ext_stores__env.
     exists sttyy. intuition. rewrite subst_rho_boolean. constructor.
-  Case "alloc_abs".
-    exists stty. intuition. rewrite subst_rho_effect. constructor.
-  Case "read_abs".
-    exists stty. intuition. rewrite subst_rho_effect. constructor.
-  Case "write_abs".
-    exists stty. intuition. rewrite subst_rho_effect. constructor.
-  Case "read_conc".
-    exists stty. intuition.
+  (* Case "alloc_abs". *)
+  - exists stty. intuition. rewrite subst_rho_effect. constructor.
+  (* Case "read_abs". *)
+  - exists stty. intuition. rewrite subst_rho_effect. constructor.
+  (* Case "write_abs". *)
+  - exists stty. intuition. rewrite subst_rho_effect. constructor.
+  (* Case "read_conc". *)
+  - exists stty. intuition.
     assert (hp = hp') by (eapply EmptyTracePreservesHeap_1; eauto; reflexivity); now subst.
     rewrite subst_rho_effect. constructor.      
-  Case "write_conc".
-    exists stty. intuition.
+  (*Case "write_conc". *)
+  - exists stty. intuition.
     assert (hp = hp') by (eapply EmptyTracePreservesHeap_1; eauto; reflexivity); now subst.
     rewrite subst_rho_effect. constructor. 
-  Case "eff_concat". exists stty. intuition. rewrite subst_rho_effect. constructor.
-  Case "eff_top". exists stty. intuition. rewrite subst_rho_effect. constructor.
-  Case "eff_empty". exists stty. intuition. rewrite subst_rho_effect. constructor.
+  (* Case "eff_concat". *)
+  - exists stty. intuition. rewrite subst_rho_effect. constructor.
+  (* Case "eff_top". *)
+  - exists stty. intuition. rewrite subst_rho_effect. constructor.
+  (*Case "eff_empty". *)
+  - exists stty. intuition. rewrite subst_rho_effect. constructor.
 Admitted.
 
 End TypeSoundness.
